Engine: Only use non-group-map Noprio semantics

Engine/NoPrioSemantics.v
@@ -14,107 +14,68 @@ From Linden Require Import FlatMap Equivalence FunctionalUtils.
 (* A rephrasing of the semantics, where priority does not matter *)
 (* It's a relation about leaves, not necessarily the first one *)
 (* There are no actions, the shape of the regex determines the relation *)
+(* For this version, we don't veen consider group_maps (although we could compute them along the way)
+   Because for the reversal property we don't need them. *)
 
 Section NoPrioSemantics.
   Context {params: LindenParameters}.
   Context (rer: RegExpRecord).
 
-  Inductive noprio: Direction -> input -> group_map -> regex -> input -> group_map -> Prop :=
+  Inductive noprio: Direction -> input -> regex -> input -> Prop :=
   | np_eps:
-    forall dir inp gm,
-      noprio dir inp gm Epsilon inp gm
+    forall dir inp,
+      noprio dir inp Epsilon inp
   | np_char:
-    forall dir inp gm cd c nextinp
+    forall dir inp cd c nextinp
       (READ: read_char rer cd inp dir = Some (c, nextinp)),
-      noprio dir inp gm (Regex.Character cd) nextinp gm
+      noprio dir inp (Regex.Character cd) nextinp
   | np_disj_left:
-    forall dir inp gm r1 r2 nextinp nextgm
-      (LEFT: noprio dir inp gm r1 nextinp nextgm),
-      noprio dir inp gm (Disjunction r1 r2) nextinp nextgm
+    forall dir inp r1 r2 nextinp
+      (LEFT: noprio dir inp r1 nextinp),
+      noprio dir inp (Disjunction r1 r2) nextinp
   | np_disj_right:
-    forall dir inp gm r1 r2 nextinp nextgm
-      (RIGHT: noprio dir inp gm r2 nextinp nextgm),
-      noprio dir inp gm (Disjunction r1 r2) nextinp nextgm
+    forall dir inp r1 r2 nextinp
+      (RIGHT: noprio dir inp r2 nextinp),
+      noprio dir inp (Disjunction r1 r2) nextinp
   | np_seq_forward:
-    forall inp0 gm0 r1 r2 inp1 gm1 inp2 gm2
-      (SEQ1: noprio forward inp0 gm0 r1 inp1 gm1)
-      (SEQ2: noprio forward inp1 gm1 r2 inp2 gm2),
-      noprio forward inp0 gm0 (Sequence r1 r2) inp2 gm2
+    forall inp0 r1 r2 inp1 inp2
+      (SEQ1: noprio forward inp0 r1 inp1)
+      (SEQ2: noprio forward inp1 r2 inp2),
+      noprio forward inp0 (Sequence r1 r2) inp2
   | np_seq_backward:
-    forall inp0 gm0 r1 r2 inp1 gm1 inp2 gm2
-      (SEQ1: noprio backward inp0 gm0 r2 inp1 gm1)
-      (SEQ2: noprio backward inp1 gm1 r1 inp2 gm2),
-      noprio backward inp0 gm0 (Sequence r1 r2) inp2 gm2
+    forall inp0 r1 r2 inp1 inp2
+      (SEQ1: noprio backward inp0 r2 inp1)
+      (SEQ2: noprio backward inp1 r1 inp2),
+      noprio backward inp0 (Sequence r1 r2) inp2
   | np_quant_forced:
-    forall dir inp0 gm0 r gidl min delta greedy inp1 gm1 inp2 gm2
-      (RESET: gidl = def_groups r)
-      (ITER: noprio dir inp0 (GroupMap.reset gidl gm0) r inp1 gm1)
-      (LOOP: noprio dir inp1 gm1 (Quantified greedy min delta r) inp2 gm2),
-      noprio dir inp0 gm0 (Quantified greedy (S min) delta r) inp2 gm2
+    forall dir inp0 r min delta greedy inp1 inp2
+      (ITER: noprio dir inp0 r inp1)
+      (LOOP: noprio dir inp1 (Quantified greedy min delta r) inp2),
+      noprio dir inp0 (Quantified greedy (S min) delta r) inp2
   | np_quant_done:
-    forall dir inp gm r greedy,
-      noprio dir inp gm (Quantified greedy 0 (NoI.N 0) r) inp gm
+    forall dir inp r greedy,
+      noprio dir inp (Quantified greedy 0 (NoI.N 0) r) inp
   | np_quant_free:
-    forall dir inp0 gm0 r greedy delta gidl inp1 gm1 inp2 gm2
-      (RESET: gidl = def_groups r)
-      (ITER: noprio dir inp0 (GroupMap.reset gidl gm0) r inp1 gm1)
+    forall dir inp0 r greedy delta inp1 inp2
+      (ITER: noprio dir inp0 r inp1)
       (PROGRESS: strict_suffix inp1 inp0 dir)
-      (LOOP: noprio dir inp1 gm1 (Quantified greedy 0 delta r) inp2 gm2),
-      noprio dir inp0 gm0 (Quantified greedy 0 (NoI.N 1 + delta)%NoI r) inp2 gm2
+      (LOOP: noprio dir inp1 (Quantified greedy 0 delta r) inp2),
+      noprio dir inp0 (Quantified greedy 0 (NoI.N 1 + delta)%NoI r) inp2
   | np_quant_skip:
-    forall dir inp gm r greedy delta,
-      noprio dir inp gm (Quantified greedy 0 (NoI.N 1 + delta)%NoI r) inp gm
+    forall dir inp r greedy delta,
+      noprio dir inp (Quantified greedy 0 (NoI.N 1 + delta)%NoI r) inp
   | np_group:
-    forall dir inp gm r gid nextinp nextgm
-      (GROUP: noprio dir inp (GroupMap.open (idx inp) gid gm) r nextinp nextgm),
-      noprio dir inp gm (Group gid r) nextinp (GroupMap.close (idx nextinp) gid nextgm)
+    forall dir inp r gid nextinp
+      (GROUP: noprio dir inp r nextinp),
+      noprio dir inp (Group gid r) nextinp
   | np_anchor:
-    forall dir inp gm a
+    forall dir inp a
       (ANCHOR: anchor_satisfied rer a inp = true),
-      noprio dir inp gm (Anchor a) inp gm.
-             
+      noprio dir inp (Anchor a) inp.
+  
   (* LATER: there will be an issue if we want to add negative lookarounds: strict positivity *)
   (* We might want to declare an oracle version of this, since this reversal is used in engines when we already know about the values of deeper lookarounds. *)
-  
-  (** * Properties  *)
-
-  (* group map irrelevance *)
-  Theorem noprio_gm_irrel:
-    forall dir inp0 gm0 r inp1 gm1 gm0'
-      (NP: noprio dir inp0 gm0 r inp1 gm1),
-    exists gm1', noprio dir inp0 gm0' r inp1 gm1'.
-  Proof.
-    intros dir inp0 gm0 r inp1 gm1 gm0' NP.
-    generalize dependent gm0'.
-    induction NP; intros.
-    - repeat (econstructor; eauto).
-    - repeat (econstructor; eauto).
-    - destruct (IHNP gm0') as [gm1' IH].
-      repeat (econstructor; eauto).
-    - destruct (IHNP gm0') as [gm1' IH].
-      solve[repeat (econstructor; eauto)].
-    - destruct (IHNP1 gm0') as [gm1' IH1].
-      destruct (IHNP2 gm1') as [gm2' IH2].
-      repeat (econstructor; eauto).
-    - destruct (IHNP1 gm0') as [gm1' IH1].
-      destruct (IHNP2 gm1') as [gm2' IH2].
-      repeat (econstructor; eauto).
-    - destruct (IHNP1 (GroupMap.reset gidl gm0')) as [gm1' IH1].
-      destruct (IHNP2 gm1') as [gm2' IH2].
-      repeat (econstructor; eauto).
-    - repeat (econstructor; eauto).
-    - destruct (IHNP1 (GroupMap.reset gidl gm0')) as [gm1' IH1].
-      destruct (IHNP2 gm1') as [gm2' IH2].
-      repeat (econstructor; eauto).
-    - eexists. apply np_quant_skip.
-    - destruct (IHNP (GroupMap.open (idx inp) gid gm0')) as [gm1' IH].
-      repeat (econstructor; eauto).
-    - repeat (econstructor; eauto).
-  Qed.
-
-  (* TODO: can we consider removing gm entirely?
-     We don't have backreferences, and we use it for reversal, the resulting group maps make no sense anyway. *)
-  
+    
   (** * NoPrio Tree Equivalence  *)
 
   Lemma two_app:
@@ -166,120 +127,124 @@ Section NoPrioSemantics.
 
   (* all leaves obtained from noprio are leaves of the backtracking tree *)
   Theorem noprio_is_leaf:
-    forall dir r inp gm t leafinp leafgm
+    forall dir r inp gm t leafinp
       (TREE: is_tree rer [Areg r] inp gm dir t),
-      noprio dir inp gm r leafinp leafgm -> 
-      In (leafinp, leafgm) (tree_leaves t gm inp dir).
+      noprio dir inp r leafinp -> 
+      exists leafgm, In (leafinp, leafgm) (tree_leaves t gm inp dir).
   Proof.
-    intros dir r inp gm t leafinp leafgm TREE NP. 
-    generalize dependent t.
+    intros dir r inp gm t leafinp TREE NP. 
+    generalize dependent t. generalize dependent gm.
     induction NP; intros.
     - inversion TREE; subst. inversion ISTREE; subst.
-      simpl. auto.
+      simpl. eauto.
     - inversion TREE; subst;
         rewrite READ0 in READ; inversion READ; subst.
       inversion TREECONT; subst. simpl.
       apply read_char_success_advance in READ0.
-      unfold advance_input'. rewrite READ0. auto.
-    - inversion TREE; subst. apply IHNP in ISTREE1.
-      simpl. apply in_or_app. auto.
-    - inversion TREE; subst. apply IHNP in ISTREE2.
-      simpl. apply in_or_app. auto.
+      unfold advance_input'. rewrite READ0. eauto.
+    - inversion TREE; subst. apply IHNP in ISTREE1 as [leafgm IH1].
+      simpl. eexists. apply in_or_app. eauto.
+    - inversion TREE; subst. apply IHNP in ISTREE2 as [leafgm IH2].
+      simpl. eexists. apply in_or_app. eauto.
     - inversion TREE; subst.
       simpl in CONT. rewrite two_app in CONT.
-      specialize (is_tree_productivity rer [Areg r1] inp0 gm0 forward) as [t1 HT1].
+      specialize (is_tree_productivity rer [Areg r1] inp0 gm forward) as [t1 HT1].
+      apply IHNP1 in HT1 as H. destruct H as [gm1 IN1].
       specialize (is_tree_productivity rer [Areg r2] inp1 gm1 forward) as [t2 HT2].
-      eapply in_leaves_app; eauto.
+      apply IHNP2 in HT2 as H. destruct H as [gm2 IN2].
+      eexists. eapply in_leaves_app; eauto.
     - inversion TREE; subst.
       simpl in CONT. rewrite two_app in CONT.
-      specialize (is_tree_productivity rer [Areg r2] inp0 gm0 backward) as [t1 HT1].
-      specialize (is_tree_productivity rer [Areg r1] inp1 gm1 backward) as [t2 HT2].
-      eapply in_leaves_app; eauto.
+      specialize (is_tree_productivity rer [Areg r2] inp0 gm backward) as [t2 HT2].
+      apply IHNP1 in HT2 as H. destruct H as [gm2 IN2].
+      specialize (is_tree_productivity rer [Areg r1] inp1 gm2 backward) as [t1 HT1].
+      apply IHNP2 in HT1 as H. destruct H as [gm1 IN1].
+      eexists. eapply in_leaves_app; eauto.
     - inversion TREE; subst.
       rewrite two_app in ISTREE1.
-      specialize (is_tree_productivity rer [Areg r] inp0 (GroupMap.reset (def_groups r) gm0) dir) as [t1 HT1].
+      specialize (is_tree_productivity rer [Areg r] inp0 (GroupMap.reset (def_groups r) gm) dir) as [t1 HT1].
+      assert (IN1: exists gm1, In (inp1, gm1) (tree_leaves t1 (GroupMap.reset (def_groups r) gm) inp0 dir)).
+      { apply IHNP1. auto. } destruct IN1 as [gm1 IN1].
       specialize (is_tree_productivity rer [Areg (Quantified greedy min delta r)] inp1 gm1 dir) as [t2 HT2].
-      assert (IN1: In (inp1, gm1) (tree_leaves t1 (GroupMap.reset (def_groups r) gm0) inp0 dir)).
-      { apply IHNP1. auto. }
-      assert (IN2: In (inp2, gm2) (tree_leaves t2 gm1 inp1 dir)).
-      { apply IHNP2. auto. }
-      eapply (in_leaves_app _ _ _ _ _ inp2 gm2 _ _ _ _ _ ISTREE1 HT1 HT2 IN1 IN2); eauto.
+      assert (IN2: exists gm2, In (inp2, gm2) (tree_leaves t2 gm1 inp1 dir)).
+      { apply IHNP2. auto. } destruct IN2 as [gm2 IN2].
+      eexists. eapply (in_leaves_app _ _ _ _ _ inp2 gm2 _ _ _ _ _ ISTREE1 HT1 HT2 IN1 IN2); eauto.
     - inversion TREE; subst.
-      + inversion SKIP; subst. simpl. auto.
+      + inversion SKIP; subst. simpl. eauto.
       + destruct plus; inversion H1.
     - inversion TREE; subst.
       { destruct delta; inversion H1. }
       assert (DP: plus = delta).
       { destruct plus; destruct delta; auto; inversion H1; auto. }
       subst. clear H1. clear SKIP.
-      specialize (is_tree_productivity rer [Areg r] inp0 (GroupMap.reset (def_groups r) gm0) dir) as [t1 HT1].
+      specialize (is_tree_productivity rer [Areg r] inp0 (GroupMap.reset (def_groups r) gm) dir) as [t1 HT1].
+      assert (IN1: exists gm1, In (inp1, gm1) (tree_leaves t1 (GroupMap.reset (def_groups r) gm) inp0 dir)).
+      { apply IHNP1. auto. } destruct IN1 as [gm1 IN1].
       specialize (is_tree_productivity rer [Acheck inp0] inp1 gm1 dir) as [t2 HT2].
-      specialize (is_tree_productivity rer [Areg (Quantified greedy 0 delta r)] inp1 gm1 dir) as [t3 HT3].
-      assert (IN1: In (inp1, gm1) (tree_leaves t1 (GroupMap.reset (def_groups r) gm0) inp0 dir)).
-      { apply IHNP1. auto. }
       assert (IN2: In (inp1, gm1) (tree_leaves t2 gm1 inp1 dir)).
       { inversion HT2; subst.
         - inversion TREECONT; subst. simpl. auto.
         - apply CHECKFAIL in PROGRESS. inversion PROGRESS. (* we know progress happened *)
       }
-      assert (IN3: In (inp2, gm2) (tree_leaves t3 gm1 inp1 dir)).
-      { apply IHNP2. auto. }
+      specialize (is_tree_productivity rer [Areg (Quantified greedy 0 delta r)] inp1 gm1 dir) as [t3 HT3].      
+      assert (IN3: exists gm2, In (inp2, gm2) (tree_leaves t3 gm1 inp1 dir)).
+      { apply IHNP2. auto. } destruct IN3 as [gm2 IN3].
       rewrite three_app in ISTREE1.
       destruct greedy; simpl.
-      + apply in_or_app. left.
+      + eexists. apply in_or_app. left.
         eapply (in_leaves_app3 _ _ _ _ _ _ _ _ _ _ _ _ _ _ _ _ ISTREE1 HT1 HT2 HT3 IN1 IN2 IN3). 
-      + apply in_or_app. right.
+      + eexists. apply in_or_app. right.
         eapply (in_leaves_app3 _ _ _ _ _ _ _ _ _ _ _ _ _ _ _ _ ISTREE1 HT1 HT2 HT3 IN1 IN2 IN3). 
     - inversion TREE; subst.
       { destruct delta; inversion H1. }
       inversion SKIP. subst.
-      destruct greedy; simpl; auto.
-      apply in_or_app; simpl; auto.      
+      destruct greedy; simpl; eauto.
+      eexists. apply in_or_app; simpl; eauto.      
     - inversion TREE; subst.
       rewrite two_app in TREECONT.
       specialize (is_tree_productivity rer [Areg r] inp (GroupMap.open (idx inp) gid gm) dir) as [t1 HT1].
+      assert (IN1: exists nextgm, In (nextinp, nextgm) (tree_leaves t1 (GroupMap.open (idx inp) gid gm) inp dir)).
+      { apply IHNP. auto. } destruct IN1 as [nextgm IN1].
       specialize (is_tree_productivity rer [Aclose gid] nextinp nextgm dir) as [t2 HT2].
-      assert (IN1: In (nextinp, nextgm) (tree_leaves t1 (GroupMap.open (idx inp) gid gm) inp dir)).
-      { apply IHNP. auto. }
       assert (IN2: In (nextinp, GroupMap.close (idx nextinp) gid nextgm) (tree_leaves t2 nextgm nextinp dir)).
       { inversion HT2. subst. inversion TREECONT0. subst. simpl. auto. }
-      eapply (in_leaves_app _ _ _ _ _ nextinp (GroupMap.close (idx nextinp) gid nextgm) _ _ _ _ _ TREECONT HT1 HT2 IN1 IN2); eauto.
+      eexists. eapply (in_leaves_app _ _ _ _ _ nextinp (GroupMap.close (idx nextinp) gid nextgm) _ _ _ _ _ TREECONT HT1 HT2 IN1 IN2); eauto.
     - inversion TREE; subst;
         rewrite ANCHOR0 in ANCHOR; inversion ANCHOR.
-      inversion TREECONT; subst. simpl. auto.
+      inversion TREECONT; subst. simpl. eauto.
   Qed.
 
   (* Other direction: generalizing the noprio semantics to actions *)
 
-  Inductive noprio_action: Direction -> input -> group_map -> action -> input -> group_map -> Prop :=
+  Inductive noprio_action: Direction -> input -> action -> input -> Prop :=
   | np_regex:
-    forall dir inp gm r nextinp nextgm
-      (NP: noprio dir inp gm r nextinp nextgm),
-      noprio_action dir inp gm (Areg r) nextinp nextgm
+    forall dir inp r nextinp
+      (NP: noprio dir inp r nextinp),
+      noprio_action dir inp (Areg r) nextinp
   | np_close:
-    forall dir inp gm gid,
-      noprio_action dir inp gm (Aclose gid) inp (GroupMap.close (idx inp) gid gm)
+    forall dir inp gid,
+      noprio_action dir inp (Aclose gid) inp
   | np_check:
-    forall dir inp gm inpcheck
+    forall dir inp inpcheck
       (PROGRESS: strict_suffix inp inpcheck dir),
-      noprio_action dir inp gm (Acheck inpcheck) inp gm.
+      noprio_action dir inp (Acheck inpcheck) inp.
 
-  Inductive noprio_list: Direction -> input -> group_map -> list action -> input -> group_map -> Prop :=
+  Inductive noprio_list: Direction -> input -> list action -> input -> Prop :=
   | np_nil:
-    forall dir inp gm,
-      noprio_list dir inp gm [] inp gm
+    forall dir inp,
+      noprio_list dir inp [] inp
   | np_cons:
-    forall dir inp0 gm0 a inp1 gm1 l inp2 gm2
-      (NP_A: noprio_action dir inp0 gm0 a inp1 gm1)
-      (NP_L: noprio_list dir inp1 gm1 l inp2 gm2),
-      noprio_list dir inp0 gm0 (a::l) inp2 gm2.
+    forall dir inp0 a inp1 l inp2
+      (NP_A: noprio_action dir inp0 a inp1)
+      (NP_L: noprio_list dir inp1 l inp2),
+      noprio_list dir inp0 (a::l) inp2.
 
   Lemma is_tree_action_noprio:
     forall dir inp0 gm0 l t inp1 gm1
       (SUBSET: pike_actions l)
       (TREE: is_tree rer l inp0 gm0 dir t)
       (LEAF: In (inp1, gm1) (tree_leaves t gm0 inp0 dir)),
-      noprio_list dir inp0 gm0 l inp1 gm1.
+      noprio_list dir inp0 l inp1.
   Proof.
     intros dir inp0 gm0 l t inp1 gm1 SUBSET TREE LEAF.
     induction TREE; simpl in LEAF; subst;
@@ -293,20 +258,20 @@ Section NoPrioSemantics.
            unfold advance_input' in LEAF. rewrite ADV in LEAF. eauto. }
       repeat (econstructor; eauto). 
     - apply in_app_or in LEAF as [LEAF|LEAF].
-      + assert (noprio_list dir inp gm (Areg r1::cont) inp1 gm1).
+      + assert (noprio_list dir inp (Areg r1::cont) inp1).
         { apply IHTREE1; auto. pike_subset. }
         inversion H; subst. inversion NP_A. repeat (econstructor; eauto).
-      + assert (noprio_list dir inp gm (Areg r2::cont) inp1 gm1).
+      + assert (noprio_list dir inp (Areg r2::cont) inp1).
         { apply IHTREE2; auto. pike_subset. }
         inversion H; subst. inversion NP_A. solve[repeat (econstructor; eauto)].
     - destruct dir.
       + simpl in IHTREE.
-        assert (noprio_list forward inp gm (Areg r1 :: Areg r2 :: cont) inp1 gm1).
+        assert (noprio_list forward inp (Areg r1 :: Areg r2 :: cont) inp1).
         { apply IHTREE; auto. pike_subset. }
         inversion H; inversion NP_L; inversion NP_A; inversion NP_A0; subst.
         repeat (econstructor; eauto).
       + simpl in IHTREE.
-        assert (noprio_list backward inp gm (Areg r2 :: Areg r1 :: cont) inp1 gm1).
+        assert (noprio_list backward inp (Areg r2 :: Areg r1 :: cont) inp1).
         { apply IHTREE; auto. pike_subset. }
         inversion H; inversion NP_L; inversion NP_A; inversion NP_A0; subst.
         repeat (econstructor; eauto).
@@ -321,7 +286,7 @@ Section NoPrioSemantics.
       (* skip *)
       2: { econstructor; eauto. econstructor; eauto. apply np_quant_skip. }
       (* iter *)
-      assert (noprio_list dir inp (GroupMap.reset (def_groups r1) gm) (Areg r1 :: Acheck inp :: Areg (Quantified greedy 0 +∞ r1) :: cont) inp1 gm1).
+      assert (noprio_list dir inp (Areg r1 :: Acheck inp :: Areg (Quantified greedy 0 +∞ r1) :: cont) inp1).
       { apply IHTREE1; auto. pike_subset. }
       inversion H; inversion NP_L; inversion NP_A; inversion NP_A0; inversion NP_L0; inversion NP_A1; subst.
       repeat (econstructor; eauto).
@@ -334,12 +299,12 @@ Section NoPrioSemantics.
       (* skip *)
       2: { econstructor; eauto. econstructor; eauto. apply np_quant_skip. }
       (* iter *)
-      assert (noprio_list dir inp (GroupMap.reset (def_groups r1) gm) (Areg r1 :: Acheck inp :: Areg (Quantified greedy 0 (NoI.N 0) r1) :: cont) inp1 gm1).
+      assert (noprio_list dir inp (Areg r1 :: Acheck inp :: Areg (Quantified greedy 0 (NoI.N 0) r1) :: cont) inp1).
       { apply IHTREE1; auto. pike_subset. }
       inversion H; inversion NP_L; inversion NP_A; inversion NP_A0; inversion NP_L0; inversion NP_A1; subst.
       repeat (econstructor; eauto).
     - destruct plus; inversion H3.
-    - assert (noprio_list dir inp (GroupMap.open (idx inp) gid gm) (Areg r1 :: Aclose gid :: cont) inp1 gm1).
+    - assert (noprio_list dir inp (Areg r1 :: Aclose gid :: cont) inp1).
       { apply IHTREE; auto. pike_subset. }
       inversion H; inversion NP_A; inversion NP_L; inversion NP_A0; subst.
       repeat (econstructor; eauto).
@@ -349,19 +314,126 @@ Section NoPrioSemantics.
 
   (* For the Pike Subset, the NoPrio Semantics exactly coincides with leaves of the Tree Semantics *)
   Theorem noprio_eq_is_leaf:
-    forall dir r inp gm t leafinp leafgm
+    forall dir r inp gm t leafinp
       (SUBSET: pike_regex r)
       (TREE: is_tree rer [Areg r] inp gm dir t),
-      noprio dir inp gm r leafinp leafgm <-> 
-        In (leafinp, leafgm) (tree_leaves t gm inp dir).
+      noprio dir inp r leafinp <-> 
+        exists leafgm, In (leafinp, leafgm) (tree_leaves t gm inp dir).
   Proof.
-    intros dir r inp gm t leafinp leafgm SUBSET TREE. split.
+    intros dir r inp gm t leafinp SUBSET TREE. split.
     - apply noprio_is_leaf. auto.
-    - intros. eapply is_tree_action_noprio in TREE; eauto.
+    - intros [leafgm H]. eapply is_tree_action_noprio in TREE; eauto.
       2: pike_subset.
       inversion TREE; inversion NP_A; inversion NP_L; subst. auto.
   Qed.
 
+  (** * Quantifier Properties  *)
+
+  Lemma iteration_suffix:
+    forall dir r inp0 inp1
+      (NP: noprio dir inp0 r inp1),
+      inp0 = inp1 \/ strict_suffix inp1 inp0 dir.
+  Proof.
+    intros dir r inp0 inp1 NP. induction NP; auto.
+    1: { apply read_char_suffix in READ. auto. }
+    all: destruct IHNP1; destruct IHNP2; subst; auto;
+      right; eapply strict_suffix_trans; eauto.
+  Qed.
+
+  (* In order to prove the reversal property, we characterize quantifiers in the nopriority semantics *)
+
+  (* n iterations of a regex *)
+  Inductive iters : nat -> Direction -> input -> regex -> input -> Prop :=
+  | iters_refl:
+    forall inp r dir, iters 0 dir inp r inp
+  | iters_next:
+    forall r n inp0 inp1 inp2 dir
+      (NEXT: noprio dir inp0 r inp1)
+      (ITERS: iters n dir inp1 r inp2),
+      iters (S n) dir inp0 r inp2.
+
+  (* is n <= min + delta ? *)
+  Inductive smaller: nat -> nat -> non_neg_integer_or_inf -> Prop :=
+  | smaller_nat: forall n min delta,
+      n <= min + delta ->
+      smaller n min (NoI.N delta)
+  | smaller_inf: forall n min,
+      smaller n min NoI.Inf.
+
+  (* a characterization of quantifiers using numbered iterations *)
+  Lemma quant_iters:
+     forall r dir greedy inp0 inp1 min delta
+      (QUANT: noprio dir inp0 (Quantified greedy min delta r) inp1),
+     exists n, n >= min /\ smaller n min delta /\ iters n dir inp0 r inp1.
+  Proof.
+    intros r dir greedy inp0 inp1 min delta QUANT.
+    remember (Quantified greedy min delta r) as quant.
+    generalize dependent min. generalize dependent delta.
+    induction QUANT; intros; 
+      inversion Heqquant; subst.
+    - clear IHQUANT1.
+      specialize (IHQUANT2 delta0 min (eq_refl _)) as [n [GE [LE IT]]].
+      exists (S n). split; [lia|]. split.
+      { inversion LE; subst; constructor. lia. }
+      econstructor; eauto.
+    - exists 0. split; [lia|]. split; constructor; auto.
+    - clear IHQUANT1. specialize (IHQUANT2 delta 0 (eq_refl _)) as [n [GE [LE IT]]].
+      exists (S n). split; [lia|]. split.
+      { inversion LE; subst; constructor. lia. }
+      econstructor; eauto.
+    - exists 0. split; [lia|]. split.
+      { destruct delta; constructor. lia. }
+      constructor.
+  Qed.
+
+  Lemma iters_quant:
+    forall r dir greedy inp0 inp1 min delta n
+      (GE: n >= min)
+      (LE: smaller n min delta)
+      (ITERS: iters n dir inp0 r inp1),
+      noprio dir inp0 (Quantified greedy min delta r) inp1.
+  Proof.
+    intros r dir greedy inp0 inp1 min delta n GE LE ITERS.
+    generalize dependent min. generalize dependent delta.
+    induction ITERS; intros.
+    - destruct min; inversion GE. inversion LE; subst.
+      + destruct delta0.
+        * apply np_quant_done.
+        * replace (NoI.N (S delta0)) with (NoI.N 1 + NoI.N delta0)%NoI by auto.
+          apply np_quant_skip.
+      + replace NoI.Inf with (NoI.N 1 + NoI.Inf)%NoI by auto.
+        apply np_quant_skip.
+    - destruct min.
+      (* forced iteration *)
+      2:{ eapply np_quant_forced; eauto. apply IHITERS. lia.
+          inversion LE; subst; constructor. lia. }
+    (* free iteration: cas analysis on if the first iteration did progress   *)
+      apply iteration_suffix in NEXT as H. destruct H as [EQ|SUF].
+      + (* first iteration didn't progress: we skip it in the quantifier *)
+        subst. apply IHITERS. lia. inversion LE; subst; constructor. lia.
+      + (* first iteration made progress: we can use it as a quantifier iteration *)
+        inversion LE; subst.
+        * destruct delta0; [lia|].
+          replace (NoI.N (S delta0)) with (NoI.N 1 + NoI.N delta0)%NoI by auto.
+          eapply np_quant_free; eauto. apply IHITERS. lia.
+          constructor. lia.
+        * replace NoI.Inf with (NoI.N 1 + NoI.Inf)%NoI by auto.
+          eapply np_quant_free; eauto. apply IHITERS. lia.
+          constructor.
+  Qed.
+
+  (* Adding an iteration at the end *)
+  Lemma add_iter_end:
+    forall dir r n inp0 inp1 inp2
+      (ITERS: iters n dir inp0 r inp1)
+      (NEXT: noprio dir inp1 r inp2),
+      iters (S n) dir inp0 r inp2.
+  Proof.
+    intros. induction ITERS; repeat (econstructor; eauto).
+  Qed.
+
+      
+  
   (** * Reversal Property  *)
 
   Definition reverse (d:Direction): Direction :=
@@ -384,75 +456,54 @@ Section NoPrioSemantics.
       destruct (char_match) eqn:CM; inversion H. subst.
       rewrite CM. auto.
   Qed.
-
-  Theorem noprio_reversal:
-    forall dir r inp1 inp2 gma gmb
-      (NP1: noprio dir inp1 gma r inp2 gmb),
-    forall gmc, exists gmd, noprio (reverse dir) inp2 gmc r inp1 gmd.
-  Proof.
-    intros dir r.
-    induction r; intros.
-    - inversion NP1. subst. repeat (econstructor; eauto).
-    - inversion NP1. subst.
-      apply read_char_reverse in READ as REV.
-      repeat (econstructor; eauto).
-    - inversion NP1; subst.
-      + eapply IHr1 in LEFT as [gmd H]. repeat (econstructor; eauto).
-      + eapply IHr2 in RIGHT as [gmd H]. solve[repeat (econstructor; eauto)].
-    - inversion NP1; subst; simpl in *.
-      + apply IHr2 with (gmc:=gmc) in SEQ2 as [gmd H2].
-        apply IHr1 with (gmc:=gmd) in SEQ1 as H1. destruct H1 as [gme H1].
-        (* ah! why doesn't the intro pattern work here? *)
-        repeat (econstructor; eauto).
-      + apply IHr1 with (gmc:=gmc) in SEQ2 as [gmd H2].
-        apply IHr2 with (gmc:=gmd) in SEQ1 as H1. destruct H1 as [gme H1].
-        repeat (econstructor; eauto).
-    - inversion NP1; subst.
-      +                         (* forced *)
-      (* induction over r fails: r{min} is not a subregex of r{min+1} *)
-        admit.
-      +                         (* done *)
-        repeat (econstructor; eauto).
-      +                         (* free *)
-        admit.
-      +                         (* skip *)
-        exists gmc. apply np_quant_skip.
-    - inversion NP1.
-    - inversion NP1. subst.
-      eapply IHr in GROUP as [gmd H].
-      repeat (econstructor; eauto).
-    - inversion NP1. subst.
-      repeat (econstructor; eauto).
-    - inversion NP1.
-  Abort.
-
   
   Theorem noprio_reversal:
-    forall dir r inp1 inp2 gma gmb
-      (NP1: noprio dir inp1 gma r inp2 gmb),
-    forall gmc, exists gmd, noprio (reverse dir) inp2 gmc r inp1 gmd.
+    forall dir r inp1 inp2
+      (NP1: noprio dir inp1 r inp2),
+      noprio (reverse dir) inp2 r inp1.
   Proof.
-    intros dir r inp1 inp2 gma gmb NP1 gmc.
-    generalize dependent gmc. induction NP1; intros.
+    intros dir r inp1 inp2 NP1.
+    induction NP1; intros.
     - repeat (econstructor; eauto).
     - apply read_char_reverse in READ as REV.
-      destruct dir; simpl; exists gmc; econstructor; eauto.
-    - destruct (IHNP1 gmc) as [gmd H]. eexists. apply np_disj_left. eauto.
-    - destruct (IHNP1 gmc) as [gmd H]. eexists. apply np_disj_right. eauto.
-    - destruct (IHNP1_2 gmc) as [gmd H2]. destruct (IHNP1_1 gmd) as [gme H1].
-      repeat (econstructor; eauto).
-    - destruct (IHNP1_2 gmc) as [gmd H1]. destruct (IHNP1_1 gmd) as [gme H2].
-      repeat (econstructor; eauto).
-    - admit.
-    (* does not work: in one direction we do r and then r{min}
-       in the other we also do r and then r{min}, but we would like them switched to apply IH.
-       One solution would be to prove that for noprio, r.r{} is equivalent to r{}.r *)
+      destruct dir; simpl; econstructor; eauto.
+    - repeat (econstructor; eauto). 
+    - solve[repeat (econstructor; eauto)].
     - repeat (econstructor; eauto).
-    - admit.
-    - eexists. eapply np_quant_skip.
-    - destruct (IHNP1 (GroupMap.open (idx nextinp) gid gmc)) as [gmd H1].
-      repeat (econstructor; eauto).
     - repeat (econstructor; eauto).
-  Admitted.
+    - apply quant_iters in IHNP1_2 as [n [GE [LE IT]]].
+      apply iters_quant with (n:= S n); auto. lia.
+      { inversion LE; subst; constructor. lia. }
+      eapply add_iter_end; eauto.
+    - repeat (econstructor; eauto).
+    - apply quant_iters in IHNP1_2 as [n [GE [LE IT]]].
+      apply iters_quant with (n:=S n); auto.
+      { inversion LE; subst; constructor. lia. }
+      eapply add_iter_end; eauto.
+    - eapply np_quant_skip.
+    - repeat (econstructor; eauto).
+    - repeat (econstructor; eauto).
+  Qed.
+
+  (** * Leaf Reversal Theorem  *)
+
+  (* We come back to is_tree semantics to prove the reversal property *)
   
+  Lemma leaf_reversal:
+    forall r dir inp1 inp2 gm2 t1 t2
+      (SUBSET: pike_regex r)
+      (TREE1: is_tree rer [Areg r] inp1 GroupMap.empty dir t1)
+      (TREE2: is_tree rer [Areg r] inp2 GroupMap.empty (reverse dir) t2)
+      (IN: In (inp2, gm2) (tree_leaves t1 GroupMap.empty inp1 dir)),
+    exists gm1, In (inp1, gm1) (tree_leaves t2 GroupMap.empty inp2 (reverse dir)).
+  Proof.
+    intros r dir inp1 inp2 gm2 t1 t2 SUBSET TREE1 TREE2 IN.
+    assert (NP1: noprio dir inp1 r inp2).
+    { apply <- noprio_eq_is_leaf; eauto. }
+    apply noprio_reversal in NP1 as NP2.
+    assert (IN2: exists leafgm, In (inp1, leafgm) (tree_leaves t2 GroupMap.empty inp2 (reverse dir))).
+    { eapply noprio_eq_is_leaf; eauto. }
+    eauto.
+  Qed.
+    
 End NoPrioSemantics.
